rewrite for forall descend under the binder, extending the vprop_equiv relation

pulse/src/ocaml/plugin/generated/Pulse_Main.ml
@@ -143,7 +143,7 @@ let (check_fndecl :
             (FStar_Sealed.seal
                (Obj.magic
                   (FStar_Range.mk_range "Pulse.Main.fst" (Prims.of_int (46))
-                     Prims.int_one (Prims.of_int (107)) (Prims.of_int (30)))))
+                     Prims.int_one (Prims.of_int (109)) (Prims.of_int (30)))))
             (FStar_Tactics_Effect.lift_div_tac
                (fun uu___ -> d.Pulse_Syntax_Base.d))
             (fun uu___ ->
@@ -161,7 +161,7 @@ let (check_fndecl :
                               (Obj.magic
                                  (FStar_Range.mk_range "Pulse.Main.fst"
                                     (Prims.of_int (50)) (Prims.of_int (46))
-                                    (Prims.of_int (107)) (Prims.of_int (30)))))
+                                    (Prims.of_int (109)) (Prims.of_int (30)))))
                            (FStar_Tactics_Effect.lift_div_tac
                               (fun uu___1 ->
                                  FStar_Pervasives_Native.fst
@@ -185,7 +185,7 @@ let (check_fndecl :
                                                "Pulse.Main.fst"
                                                (Prims.of_int (55))
                                                (Prims.of_int (4))
-                                               (Prims.of_int (107))
+                                               (Prims.of_int (109))
                                                (Prims.of_int (30)))))
                                       (if fn_d.Pulse_Syntax_Base.isrec
                                        then
@@ -216,7 +216,7 @@ let (check_fndecl :
                                                           "Pulse.Main.fst"
                                                           (Prims.of_int (55))
                                                           (Prims.of_int (4))
-                                                          (Prims.of_int (107))
+                                                          (Prims.of_int (109))
                                                           (Prims.of_int (30)))))
                                                  (FStar_Tactics_Effect.lift_div_tac
                                                     (fun uu___1 ->
@@ -255,7 +255,7 @@ let (check_fndecl :
                                                                     "Pulse.Main.fst"
                                                                     (Prims.of_int (60))
                                                                     (Prims.of_int (2))
-                                                                    (Prims.of_int (107))
+                                                                    (Prims.of_int (109))
                                                                     (Prims.of_int (30)))))
                                                                 (FStar_Tactics_Effect.lift_div_tac
                                                                    (fun
@@ -283,7 +283,7 @@ let (check_fndecl :
                                                                     "Pulse.Main.fst"
                                                                     (Prims.of_int (61))
                                                                     (Prims.of_int (63))
-                                                                    (Prims.of_int (107))
+                                                                    (Prims.of_int (109))
                                                                     (Prims.of_int (30)))))
                                                                     (if
                                                                     Prims.uu___is_Nil
@@ -323,7 +323,7 @@ let (check_fndecl :
                                                                     "Pulse.Main.fst"
                                                                     (Prims.of_int (62))
                                                                     (Prims.of_int (37))
-                                                                    (Prims.of_int (107))
+                                                                    (Prims.of_int (109))
                                                                     (Prims.of_int (30)))))
                                                                     (Obj.magic
                                                                     (mk_abs g
@@ -347,9 +347,9 @@ let (check_fndecl :
                                                                     (Obj.magic
                                                                     (FStar_Range.mk_range
                                                                     "Pulse.Main.fst"
-                                                                    (Prims.of_int (63))
-                                                                    (Prims.of_int (25))
-                                                                    (Prims.of_int (107))
+                                                                    (Prims.of_int (64))
+                                                                    (Prims.of_int (2))
+                                                                    (Prims.of_int (109))
                                                                     (Prims.of_int (30)))))
                                                                     (FStar_Tactics_Effect.lift_div_tac
                                                                     (fun
@@ -366,26 +366,83 @@ let (check_fndecl :
                                                                     (FStar_Range.mk_range
                                                                     "Pulse.Main.fst"
                                                                     (Prims.of_int (64))
-                                                                    (Prims.of_int (32))
+                                                                    (Prims.of_int (2))
                                                                     (Prims.of_int (64))
+                                                                    (Prims.of_int (96)))))
+                                                                    (FStar_Sealed.seal
+                                                                    (Obj.magic
+                                                                    (FStar_Range.mk_range
+                                                                    "Pulse.Main.fst"
+                                                                    (Prims.of_int (64))
+                                                                    (Prims.of_int (97))
+                                                                    (Prims.of_int (109))
+                                                                    (Prims.of_int (30)))))
+                                                                    (Obj.magic
+                                                                    (debug_main
+                                                                    g
+                                                                    (fun
+                                                                    uu___3 ->
+                                                                    FStar_Tactics_Effect.tac_bind
+                                                                    (FStar_Sealed.seal
+                                                                    (Obj.magic
+                                                                    (FStar_Range.mk_range
+                                                                    "Pulse.Main.fst"
+                                                                    (Prims.of_int (64))
+                                                                    (Prims.of_int (69))
+                                                                    (Prims.of_int (64))
+                                                                    (Prims.of_int (95)))))
+                                                                    (FStar_Sealed.seal
+                                                                    (Obj.magic
+                                                                    (FStar_Range.mk_range
+                                                                    "prims.fst"
+                                                                    (Prims.of_int (590))
+                                                                    (Prims.of_int (19))
+                                                                    (Prims.of_int (590))
+                                                                    (Prims.of_int (31)))))
+                                                                    (Obj.magic
+                                                                    (Pulse_Syntax_Printer.st_term_to_string
+                                                                    body1))
+                                                                    (fun
+                                                                    uu___4 ->
+                                                                    FStar_Tactics_Effect.lift_div_tac
+                                                                    (fun
+                                                                    uu___5 ->
+                                                                    Prims.strcat
+                                                                    "\nbody after mk_abs:\n"
+                                                                    (Prims.strcat
+                                                                    uu___4
+                                                                    "\n"))))))
+                                                                    (fun
+                                                                    uu___3 ->
+                                                                    (fun
+                                                                    uu___3 ->
+                                                                    Obj.magic
+                                                                    (FStar_Tactics_Effect.tac_bind
+                                                                    (FStar_Sealed.seal
+                                                                    (Obj.magic
+                                                                    (FStar_Range.mk_range
+                                                                    "Pulse.Main.fst"
+                                                                    (Prims.of_int (66))
+                                                                    (Prims.of_int (32))
+                                                                    (Prims.of_int (66))
                                                                     (Prims.of_int (86)))))
                                                                     (FStar_Sealed.seal
                                                                     (Obj.magic
                                                                     (FStar_Range.mk_range
                                                                     "Pulse.Main.fst"
-                                                                    (Prims.of_int (63))
-                                                                    (Prims.of_int (25))
-                                                                    (Prims.of_int (107))
+                                                                    (Prims.of_int (64))
+                                                                    (Prims.of_int (97))
+                                                                    (Prims.of_int (109))
                                                                     (Prims.of_int (30)))))
                                                                     (Obj.magic
                                                                     (Pulse_Checker_Abs.check_abs
                                                                     g body1
                                                                     Pulse_Checker.check))
                                                                     (fun
-                                                                    uu___3 ->
+                                                                    uu___4 ->
                                                                     (fun
-                                                                    uu___3 ->
-                                                                    match uu___3
+                                                                    uu___4 ->
+                                                                    match uu___4
                                                                     with
                                                                     | 
                                                                     FStar_Pervasives.Mkdtuple3
@@ -399,64 +456,64 @@ let (check_fndecl :
                                                                     (Obj.magic
                                                                     (FStar_Range.mk_range
                                                                     "Pulse.Main.fst"
-                                                                    (Prims.of_int (66))
+                                                                    (Prims.of_int (68))
                                                                     (Prims.of_int (2))
-                                                                    (Prims.of_int (69))
+                                                                    (Prims.of_int (71))
                                                                     (Prims.of_int (35)))))
                                                                     (FStar_Sealed.seal
                                                                     (Obj.magic
                                                                     (FStar_Range.mk_range
                                                                     "Pulse.Main.fst"
-                                                                    (Prims.of_int (70))
+                                                                    (Prims.of_int (72))
                                                                     (Prims.of_int (2))
-                                                                    (Prims.of_int (107))
+                                                                    (Prims.of_int (109))
                                                                     (Prims.of_int (30)))))
                                                                     (Obj.magic
                                                                     (Pulse_Checker_Prover_Util.debug_prover
                                                                     g
                                                                     (fun
-                                                                    uu___4 ->
+                                                                    uu___5 ->
                                                                     FStar_Tactics_Effect.tac_bind
                                                                     (FStar_Sealed.seal
                                                                     (Obj.magic
                                                                     (FStar_Range.mk_range
                                                                     "Pulse.Main.fst"
-                                                                    (Prims.of_int (69))
+                                                                    (Prims.of_int (71))
                                                                     (Prims.of_int (14))
-                                                                    (Prims.of_int (69))
+                                                                    (Prims.of_int (71))
                                                                     (Prims.of_int (34)))))
                                                                     (FStar_Sealed.seal
                                                                     (Obj.magic
                                                                     (FStar_Range.mk_range
                                                                     "Pulse.Main.fst"
-                                                                    (Prims.of_int (67))
-                                                                    (Prims.of_int (14))
                                                                     (Prims.of_int (69))
+                                                                    (Prims.of_int (14))
+                                                                    (Prims.of_int (71))
                                                                     (Prims.of_int (34)))))
                                                                     (Obj.magic
                                                                     (Pulse_Syntax_Printer.comp_to_string
                                                                     c))
                                                                     (fun
-                                                                    uu___5 ->
+                                                                    uu___6 ->
                                                                     (fun
-                                                                    uu___5 ->
+                                                                    uu___6 ->
                                                                     Obj.magic
                                                                     (FStar_Tactics_Effect.tac_bind
                                                                     (FStar_Sealed.seal
                                                                     (Obj.magic
                                                                     (FStar_Range.mk_range
                                                                     "Pulse.Main.fst"
-                                                                    (Prims.of_int (67))
-                                                                    (Prims.of_int (14))
                                                                     (Prims.of_int (69))
+                                                                    (Prims.of_int (14))
+                                                                    (Prims.of_int (71))
                                                                     (Prims.of_int (34)))))
                                                                     (FStar_Sealed.seal
                                                                     (Obj.magic
                                                                     (FStar_Range.mk_range
                                                                     "Pulse.Main.fst"
-                                                                    (Prims.of_int (67))
-                                                                    (Prims.of_int (14))
                                                                     (Prims.of_int (69))
+                                                                    (Prims.of_int (14))
+                                                                    (Prims.of_int (71))
                                                                     (Prims.of_int (34)))))
                                                                     (Obj.magic
                                                                     (FStar_Tactics_Effect.tac_bind
@@ -464,9 +521,9 @@ let (check_fndecl :
                                                                     (Obj.magic
                                                                     (FStar_Range.mk_range
                                                                     "Pulse.Main.fst"
-                                                                    (Prims.of_int (68))
+                                                                    (Prims.of_int (70))
                                                                     (Prims.of_int (14))
-                                                                    (Prims.of_int (68))
+                                                                    (Prims.of_int (70))
                                                                     (Prims.of_int (40)))))
                                                                     (FStar_Sealed.seal
                                                                     (Obj.magic
@@ -480,96 +537,96 @@ let (check_fndecl :
                                                                     (Pulse_Syntax_Printer.st_term_to_string
                                                                     body2))
                                                                     (fun
-                                                                    uu___6 ->
+                                                                    uu___7 ->
                                                                     FStar_Tactics_Effect.lift_div_tac
                                                                     (fun
-                                                                    uu___7 ->
+                                                                    uu___8 ->
                                                                     fun x ->
                                                                     Prims.strcat
                                                                     (Prims.strcat
                                                                     "\ncheck call returned in main with:\n"
                                                                     (Prims.strcat
-                                                                    uu___6
+                                                                    uu___7
                                                                     "\nat type "))
                                                                     (Prims.strcat
                                                                     x "\n")))))
                                                                     (fun
-                                                                    uu___6 ->
+                                                                    uu___7 ->
                                                                     FStar_Tactics_Effect.lift_div_tac
                                                                     (fun
-                                                                    uu___7 ->
-                                                                    uu___6
-                                                                    uu___5))))
-                                                                    uu___5))))
+                                                                    uu___8 ->
+                                                                    uu___7
+                                                                    uu___6))))
+                                                                    uu___6))))
                                                                     (fun
-                                                                    uu___4 ->
+                                                                    uu___5 ->
                                                                     (fun
-                                                                    uu___4 ->
+                                                                    uu___5 ->
                                                                     Obj.magic
                                                                     (FStar_Tactics_Effect.tac_bind
                                                                     (FStar_Sealed.seal
                                                                     (Obj.magic
                                                                     (FStar_Range.mk_range
                                                                     "Pulse.Main.fst"
-                                                                    (Prims.of_int (70))
+                                                                    (Prims.of_int (72))
                                                                     (Prims.of_int (2))
-                                                                    (Prims.of_int (73))
+                                                                    (Prims.of_int (75))
                                                                     (Prims.of_int (62)))))
                                                                     (FStar_Sealed.seal
                                                                     (Obj.magic
                                                                     (FStar_Range.mk_range
                                                                     "Pulse.Main.fst"
-                                                                    (Prims.of_int (73))
+                                                                    (Prims.of_int (75))
                                                                     (Prims.of_int (63))
-                                                                    (Prims.of_int (107))
+                                                                    (Prims.of_int (109))
                                                                     (Prims.of_int (30)))))
                                                                     (Obj.magic
                                                                     (debug_main
                                                                     g
                                                                     (fun
-                                                                    uu___5 ->
+                                                                    uu___6 ->
                                                                     FStar_Tactics_Effect.tac_bind
                                                                     (FStar_Sealed.seal
                                                                     (Obj.magic
                                                                     (FStar_Range.mk_range
                                                                     "Pulse.Main.fst"
-                                                                    (Prims.of_int (73))
+                                                                    (Prims.of_int (75))
                                                                     (Prims.of_int (14))
-                                                                    (Prims.of_int (73))
+                                                                    (Prims.of_int (75))
                                                                     (Prims.of_int (61)))))
                                                                     (FStar_Sealed.seal
                                                                     (Obj.magic
                                                                     (FStar_Range.mk_range
                                                                     "Pulse.Main.fst"
-                                                                    (Prims.of_int (71))
-                                                                    (Prims.of_int (14))
                                                                     (Prims.of_int (73))
+                                                                    (Prims.of_int (14))
+                                                                    (Prims.of_int (75))
                                                                     (Prims.of_int (61)))))
                                                                     (Obj.magic
                                                                     (Pulse_Typing_Printer.print_st_typing
                                                                     g body2 c
                                                                     t_typing))
                                                                     (fun
-                                                                    uu___6 ->
+                                                                    uu___7 ->
                                                                     (fun
-                                                                    uu___6 ->
+                                                                    uu___7 ->
                                                                     Obj.magic
                                                                     (FStar_Tactics_Effect.tac_bind
                                                                     (FStar_Sealed.seal
                                                                     (Obj.magic
                                                                     (FStar_Range.mk_range
                                                                     "Pulse.Main.fst"
-                                                                    (Prims.of_int (71))
-                                                                    (Prims.of_int (14))
                                                                     (Prims.of_int (73))
+                                                                    (Prims.of_int (14))
+                                                                    (Prims.of_int (75))
                                                                     (Prims.of_int (61)))))
                                                                     (FStar_Sealed.seal
                                                                     (Obj.magic
                                                                     (FStar_Range.mk_range
                                                                     "Pulse.Main.fst"
-                                                                    (Prims.of_int (71))
-                                                                    (Prims.of_int (14))
                                                                     (Prims.of_int (73))
+                                                                    (Prims.of_int (14))
+                                                                    (Prims.of_int (75))
                                                                     (Prims.of_int (61)))))
                                                                     (Obj.magic
                                                                     (FStar_Tactics_Effect.tac_bind
@@ -577,9 +634,9 @@ let (check_fndecl :
                                                                     (Obj.magic
                                                                     (FStar_Range.mk_range
                                                                     "Pulse.Main.fst"
-                                                                    (Prims.of_int (72))
+                                                                    (Prims.of_int (74))
                                                                     (Prims.of_int (14))
-                                                                    (Prims.of_int (72))
+                                                                    (Prims.of_int (74))
                                                                     (Prims.of_int (40)))))
                                                                     (FStar_Sealed.seal
                                                                     (Obj.magic
@@ -593,56 +650,56 @@ let (check_fndecl :
                                                                     (Pulse_Syntax_Printer.st_term_to_string
                                                                     body2))
                                                                     (fun
-                                                                    uu___7 ->
+                                                                    uu___8 ->
                                                                     FStar_Tactics_Effect.lift_div_tac
                                                                     (fun
-                                                                    uu___8 ->
+                                                                    uu___9 ->
                                                                     fun x ->
                                                                     Prims.strcat
                                                                     (Prims.strcat
                                                                     "\nchecker call returned in main with:\n"
                                                                     (Prims.strcat
-                                                                    uu___7
+                                                                    uu___8
                                                                     "\nderivation="))
                                                                     (Prims.strcat
                                                                     x "\n")))))
                                                                     (fun
-                                                                    uu___7 ->
+                                                                    uu___8 ->
                                                                     FStar_Tactics_Effect.lift_div_tac
                                                                     (fun
-                                                                    uu___8 ->
-                                                                    uu___7
-                                                                    uu___6))))
-                                                                    uu___6))))
+                                                                    uu___9 ->
+                                                                    uu___8
+                                                                    uu___7))))
+                                                                    uu___7))))
                                                                     (fun
-                                                                    uu___5 ->
+                                                                    uu___6 ->
                                                                     (fun
-                                                                    uu___5 ->
+                                                                    uu___6 ->
                                                                     Obj.magic
                                                                     (FStar_Tactics_Effect.tac_bind
                                                                     (FStar_Sealed.seal
                                                                     (Obj.magic
                                                                     (FStar_Range.mk_range
                                                                     "Pulse.Main.fst"
-                                                                    (Prims.of_int (75))
+                                                                    (Prims.of_int (77))
                                                                     (Prims.of_int (15))
-                                                                    (Prims.of_int (75))
+                                                                    (Prims.of_int (77))
                                                                     (Prims.of_int (26)))))
                                                                     (FStar_Sealed.seal
                                                                     (Obj.magic
                                                                     (FStar_Range.mk_range
                                                                     "Pulse.Main.fst"
-                                                                    (Prims.of_int (75))
+                                                                    (Prims.of_int (77))
                                                                     (Prims.of_int (29))
-                                                                    (Prims.of_int (107))
+                                                                    (Prims.of_int (109))
                                                                     (Prims.of_int (30)))))
                                                                     (FStar_Tactics_Effect.lift_div_tac
                                                                     (fun
-                                                                    uu___6 ->
+                                                                    uu___7 ->
                                                                     Pulse_Elaborate_Pure.elab_comp
                                                                     c))
                                                                     (fun
-                                                                    uu___6 ->
+                                                                    uu___7 ->
                                                                     (fun
                                                                     refl_t ->
                                                                     Obj.magic
@@ -651,27 +708,27 @@ let (check_fndecl :
                                                                     (Obj.magic
                                                                     (FStar_Range.mk_range
                                                                     "Pulse.Main.fst"
-                                                                    (Prims.of_int (76))
+                                                                    (Prims.of_int (78))
                                                                     (Prims.of_int (15))
-                                                                    (Prims.of_int (76))
+                                                                    (Prims.of_int (78))
                                                                     (Prims.of_int (87)))))
                                                                     (FStar_Sealed.seal
                                                                     (Obj.magic
                                                                     (FStar_Range.mk_range
                                                                     "Pulse.Main.fst"
-                                                                    (Prims.of_int (76))
+                                                                    (Prims.of_int (78))
                                                                     (Prims.of_int (90))
-                                                                    (Prims.of_int (107))
+                                                                    (Prims.of_int (109))
                                                                     (Prims.of_int (30)))))
                                                                     (FStar_Tactics_Effect.lift_div_tac
                                                                     (fun
-                                                                    uu___6 ->
+                                                                    uu___7 ->
                                                                     Pulse_RuntimeUtils.embed_st_term_for_extraction
                                                                     body2
                                                                     (FStar_Pervasives_Native.Some
                                                                     rng)))
                                                                     (fun
-                                                                    uu___6 ->
+                                                                    uu___7 ->
                                                                     (fun
                                                                     refl_e ->
                                                                     Obj.magic
@@ -680,25 +737,25 @@ let (check_fndecl :
                                                                     (Obj.magic
                                                                     (FStar_Range.mk_range
                                                                     "Pulse.Main.fst"
-                                                                    (Prims.of_int (77))
+                                                                    (Prims.of_int (79))
                                                                     (Prims.of_int (13))
-                                                                    (Prims.of_int (77))
+                                                                    (Prims.of_int (79))
                                                                     (Prims.of_int (28)))))
                                                                     (FStar_Sealed.seal
                                                                     (Obj.magic
                                                                     (FStar_Range.mk_range
                                                                     "Pulse.Main.fst"
-                                                                    (Prims.of_int (78))
+                                                                    (Prims.of_int (80))
                                                                     (Prims.of_int (36))
-                                                                    (Prims.of_int (107))
+                                                                    (Prims.of_int (109))
                                                                     (Prims.of_int (30)))))
                                                                     (FStar_Tactics_Effect.lift_div_tac
                                                                     (fun
-                                                                    uu___6 ->
+                                                                    uu___7 ->
                                                                     ("pulse",
                                                                     refl_e)))
                                                                     (fun
-                                                                    uu___6 ->
+                                                                    uu___7 ->
                                                                     (fun blob
                                                                     ->
                                                                     Obj.magic
@@ -707,17 +764,17 @@ let (check_fndecl :
                                                                     (Obj.magic
                                                                     (FStar_Range.mk_range
                                                                     "Pulse.Main.fst"
-                                                                    (Prims.of_int (79))
+                                                                    (Prims.of_int (81))
                                                                     (Prims.of_int (17))
-                                                                    (Prims.of_int (83))
+                                                                    (Prims.of_int (85))
                                                                     (Prims.of_int (94)))))
                                                                     (FStar_Sealed.seal
                                                                     (Obj.magic
                                                                     (FStar_Range.mk_range
                                                                     "Pulse.Main.fst"
-                                                                    (Prims.of_int (84))
+                                                                    (Prims.of_int (86))
                                                                     (Prims.of_int (4))
-                                                                    (Prims.of_int (107))
+                                                                    (Prims.of_int (109))
                                                                     (Prims.of_int (30)))))
                                                                     (Obj.magic
                                                                     (FStar_Tactics_Effect.tac_bind
@@ -725,26 +782,26 @@ let (check_fndecl :
                                                                     (Obj.magic
                                                                     (FStar_Range.mk_range
                                                                     "Pulse.Main.fst"
-                                                                    (Prims.of_int (80))
+                                                                    (Prims.of_int (82))
                                                                     (Prims.of_int (13))
-                                                                    (Prims.of_int (80))
+                                                                    (Prims.of_int (82))
                                                                     (Prims.of_int (35)))))
                                                                     (FStar_Sealed.seal
                                                                     (Obj.magic
                                                                     (FStar_Range.mk_range
                                                                     "Pulse.Main.fst"
-                                                                    (Prims.of_int (81))
-                                                                    (Prims.of_int (4))
                                                                     (Prims.of_int (83))
+                                                                    (Prims.of_int (4))
+                                                                    (Prims.of_int (85))
                                                                     (Prims.of_int (94)))))
                                                                     (FStar_Tactics_Effect.lift_div_tac
                                                                     (fun
-                                                                    uu___6 ->
+                                                                    uu___7 ->
                                                                     FStar_Pervasives_Native.fst
                                                                     (FStar_Reflection_V2_Builtins.inspect_ident
                                                                     id)))
                                                                     (fun
-                                                                    uu___6 ->
+                                                                    uu___7 ->
                                                                     (fun nm
                                                                     ->
                                                                     Obj.magic
@@ -753,17 +810,17 @@ let (check_fndecl :
                                                                     (Obj.magic
                                                                     (FStar_Range.mk_range
                                                                     "Pulse.Main.fst"
-                                                                    (Prims.of_int (81))
+                                                                    (Prims.of_int (83))
                                                                     (Prims.of_int (7))
-                                                                    (Prims.of_int (81))
+                                                                    (Prims.of_int (83))
                                                                     (Prims.of_int (47)))))
                                                                     (FStar_Sealed.seal
                                                                     (Obj.magic
                                                                     (FStar_Range.mk_range
                                                                     "Pulse.Main.fst"
-                                                                    (Prims.of_int (81))
-                                                                    (Prims.of_int (4))
                                                                     (Prims.of_int (83))
+                                                                    (Prims.of_int (4))
+                                                                    (Prims.of_int (85))
                                                                     (Prims.of_int (94)))))
                                                                     (Obj.magic
                                                                     (FStar_Tactics_Effect.tac_bind
@@ -771,33 +828,33 @@ let (check_fndecl :
                                                                     (Obj.magic
                                                                     (FStar_Range.mk_range
                                                                     "Pulse.Main.fst"
-                                                                    (Prims.of_int (81))
+                                                                    (Prims.of_int (83))
                                                                     (Prims.of_int (7))
-                                                                    (Prims.of_int (81))
+                                                                    (Prims.of_int (83))
                                                                     (Prims.of_int (41)))))
                                                                     (FStar_Sealed.seal
                                                                     (Obj.magic
                                                                     (FStar_Range.mk_range
                                                                     "Pulse.Main.fst"
-                                                                    (Prims.of_int (81))
+                                                                    (Prims.of_int (83))
                                                                     (Prims.of_int (7))
-                                                                    (Prims.of_int (81))
+                                                                    (Prims.of_int (83))
                                                                     (Prims.of_int (47)))))
                                                                     (Obj.magic
                                                                     (FStar_Tactics_V2_Builtins.ext_getv
                                                                     "pulse:elab_derivation"))
                                                                     (fun
-                                                                    uu___6 ->
+                                                                    uu___7 ->
                                                                     FStar_Tactics_Effect.lift_div_tac
                                                                     (fun
-                                                                    uu___7 ->
-                                                                    uu___6 <>
+                                                                    uu___8 ->
+                                                                    uu___7 <>
                                                                     ""))))
                                                                     (fun
-                                                                    uu___6 ->
+                                                                    uu___7 ->
                                                                     (fun
-                                                                    uu___6 ->
-                                                                    if uu___6
+                                                                    uu___7 ->
+                                                                    if uu___7
                                                                     then
                                                                     Obj.magic
                                                                     (FStar_Reflection_Typing.mk_checked_let
@@ -813,10 +870,10 @@ let (check_fndecl :
                                                                     (Pulse_Typing_Env.fstar_env
                                                                     g) nm ()
                                                                     refl_t))
-                                                                    uu___6)))
-                                                                    uu___6)))
+                                                                    uu___7)))
+                                                                    uu___7)))
                                                                     (fun
-                                                                    uu___6 ->
+                                                                    uu___7 ->
                                                                     (fun
                                                                     main_decl
                                                                     ->
@@ -826,26 +883,26 @@ let (check_fndecl :
                                                                     (Obj.magic
                                                                     (FStar_Range.mk_range
                                                                     "Pulse.Main.fst"
-                                                                    (Prims.of_int (86))
+                                                                    (Prims.of_int (88))
                                                                     (Prims.of_int (17))
-                                                                    (Prims.of_int (100))
+                                                                    (Prims.of_int (102))
                                                                     (Prims.of_int (24)))))
                                                                     (FStar_Sealed.seal
                                                                     (Obj.magic
                                                                     (FStar_Range.mk_range
                                                                     "Pulse.Main.fst"
-                                                                    (Prims.of_int (101))
+                                                                    (Prims.of_int (103))
                                                                     (Prims.of_int (4))
-                                                                    (Prims.of_int (107))
+                                                                    (Prims.of_int (109))
                                                                     (Prims.of_int (30)))))
                                                                     (FStar_Tactics_Effect.lift_div_tac
                                                                     (fun
-                                                                    uu___6 ->
+                                                                    uu___7 ->
                                                                     match main_decl
                                                                     with
                                                                     | 
                                                                     (chk, se,
-                                                                    uu___7)
+                                                                    uu___8)
                                                                     ->
                                                                     (chk,
                                                                     (if
@@ -893,7 +950,7 @@ let (check_fndecl :
                                                                     (FStar_Pervasives_Native.Some
                                                                     blob))))
                                                                     (fun
-                                                                    uu___6 ->
+                                                                    uu___7 ->
                                                                     (fun
                                                                     main_decl1
                                                                     ->
@@ -903,17 +960,17 @@ let (check_fndecl :
                                                                     (Obj.magic
                                                                     (FStar_Range.mk_range
                                                                     "Pulse.Main.fst"
-                                                                    (Prims.of_int (103))
-                                                                    (Prims.of_int (4))
                                                                     (Prims.of_int (105))
+                                                                    (Prims.of_int (4))
+                                                                    (Prims.of_int (107))
                                                                     (Prims.of_int (11)))))
                                                                     (FStar_Sealed.seal
                                                                     (Obj.magic
                                                                     (FStar_Range.mk_range
                                                                     "Pulse.Main.fst"
-                                                                    (Prims.of_int (107))
+                                                                    (Prims.of_int (109))
                                                                     (Prims.of_int (2))
-                                                                    (Prims.of_int (107))
+                                                                    (Prims.of_int (109))
                                                                     (Prims.of_int (30)))))
                                                                     (if
                                                                     fn_d.Pulse_Syntax_Base.isrec
@@ -931,21 +988,22 @@ let (check_fndecl :
                                                                     (Obj.repr
                                                                     (FStar_Tactics_Effect.lift_div_tac
                                                                     (fun
-                                                                    uu___7 ->
+                                                                    uu___8 ->
                                                                     []))))
                                                                     (fun
                                                                     recursive_decls
                                                                     ->
                                                                     FStar_Tactics_Effect.lift_div_tac
                                                                     (fun
-                                                                    uu___6 ->
+                                                                    uu___7 ->
                                                                     main_decl1
                                                                     ::
                                                                     recursive_decls))))
-                                                                    uu___6)))
-                                                                    uu___6)))
-                                                                    uu___6)))
-                                                                    uu___6)))
+                                                                    uu___7)))
+                                                                    uu___7)))
+                                                                    uu___7)))
+                                                                    uu___7)))
+                                                                    uu___7)))
                                                                     uu___6)))
                                                                     uu___5)))
                                                                     uu___4)))
@@ -986,16 +1044,16 @@ let (main' :
                                (FStar_Sealed.seal
                                   (Obj.magic
                                      (FStar_Range.mk_range "Pulse.Main.fst"
-                                        (Prims.of_int (114))
+                                        (Prims.of_int (116))
                                         (Prims.of_int (6))
-                                        (Prims.of_int (115))
+                                        (Prims.of_int (117))
                                         (Prims.of_int (88)))))
                                (FStar_Sealed.seal
                                   (Obj.magic
                                      (FStar_Range.mk_range "Pulse.Main.fst"
-                                        (Prims.of_int (115))
+                                        (Prims.of_int (117))
                                         (Prims.of_int (89))
-                                        (Prims.of_int (122))
+                                        (Prims.of_int (124))
                                         (Prims.of_int (39)))))
                                (if
                                   Pulse_RuntimeUtils.debug_at_level
@@ -1008,17 +1066,17 @@ let (main' :
                                              (Obj.magic
                                                 (FStar_Range.mk_range
                                                    "Pulse.Main.fst"
-                                                   (Prims.of_int (115))
+                                                   (Prims.of_int (117))
                                                    (Prims.of_int (16))
-                                                   (Prims.of_int (115))
+                                                   (Prims.of_int (117))
                                                    (Prims.of_int (88)))))
                                           (FStar_Sealed.seal
                                              (Obj.magic
                                                 (FStar_Range.mk_range
                                                    "Pulse.Main.fst"
-                                                   (Prims.of_int (115))
+                                                   (Prims.of_int (117))
                                                    (Prims.of_int (8))
-                                                   (Prims.of_int (115))
+                                                   (Prims.of_int (117))
                                                    (Prims.of_int (88)))))
                                           (Obj.magic
                                              (FStar_Tactics_Effect.tac_bind
@@ -1026,9 +1084,9 @@ let (main' :
                                                    (Obj.magic
                                                       (FStar_Range.mk_range
                                                          "Pulse.Main.fst"
-                                                         (Prims.of_int (115))
+                                                         (Prims.of_int (117))
                                                          (Prims.of_int (67))
-                                                         (Prims.of_int (115))
+                                                         (Prims.of_int (117))
                                                          (Prims.of_int (87)))))
                                                 (FStar_Sealed.seal
                                                    (Obj.magic
@@ -1066,17 +1124,17 @@ let (main' :
                                              (Obj.magic
                                                 (FStar_Range.mk_range
                                                    "Pulse.Main.fst"
-                                                   (Prims.of_int (116))
+                                                   (Prims.of_int (118))
                                                    (Prims.of_int (38))
-                                                   (Prims.of_int (116))
+                                                   (Prims.of_int (118))
                                                    (Prims.of_int (84)))))
                                           (FStar_Sealed.seal
                                              (Obj.magic
                                                 (FStar_Range.mk_range
                                                    "Pulse.Main.fst"
-                                                   (Prims.of_int (115))
+                                                   (Prims.of_int (117))
                                                    (Prims.of_int (89))
-                                                   (Prims.of_int (122))
+                                                   (Prims.of_int (124))
                                                    (Prims.of_int (39)))))
                                           (Obj.magic
                                              (Pulse_Checker_Pure.compute_tot_term_type
@@ -1092,17 +1150,17 @@ let (main' :
                                                             (Obj.magic
                                                                (FStar_Range.mk_range
                                                                   "Pulse.Main.fst"
-                                                                  (Prims.of_int (117))
+                                                                  (Prims.of_int (119))
                                                                   (Prims.of_int (6))
-                                                                  (Prims.of_int (118))
+                                                                  (Prims.of_int (120))
                                                                   (Prims.of_int (80)))))
                                                          (FStar_Sealed.seal
                                                             (Obj.magic
                                                                (FStar_Range.mk_range
                                                                   "Pulse.Main.fst"
-                                                                  (Prims.of_int (118))
+                                                                  (Prims.of_int (120))
                                                                   (Prims.of_int (81))
-                                                                  (Prims.of_int (122))
+                                                                  (Prims.of_int (124))
                                                                   (Prims.of_int (39)))))
                                                          (if
                                                             Prims.op_Negation
@@ -1135,18 +1193,18 @@ let (main' :
                                                                     (Obj.magic
                                                                     (FStar_Range.mk_range
                                                                     "Pulse.Main.fst"
-                                                                    (Prims.of_int (119))
+                                                                    (Prims.of_int (121))
                                                                     (Prims.of_int (51))
-                                                                    (Prims.of_int (119))
+                                                                    (Prims.of_int (121))
                                                                     (Prims.of_int (61)))))
                                                                     (
                                                                     FStar_Sealed.seal
                                                                     (Obj.magic
                                                                     (FStar_Range.mk_range
                                                                     "Pulse.Main.fst"
-                                                                    (Prims.of_int (120))
-                                                                    (Prims.of_int (6))
                                                                     (Prims.of_int (122))
+                                                                    (Prims.of_int (6))
+                                                                    (Prims.of_int (124))
                                                                     (Prims.of_int (39)))))
                                                                     (
                                                                     FStar_Tactics_Effect.lift_div_tac
@@ -1178,36 +1236,36 @@ let (join_smt_goals : unit -> (unit, unit) FStar_Tactics_Effect.tac_repr) =
     FStar_Tactics_Effect.tac_bind
       (FStar_Sealed.seal
          (Obj.magic
-            (FStar_Range.mk_range "Pulse.Main.fst" (Prims.of_int (128))
-               (Prims.of_int (2)) (Prims.of_int (129)) (Prims.of_int (35)))))
+            (FStar_Range.mk_range "Pulse.Main.fst" (Prims.of_int (130))
+               (Prims.of_int (2)) (Prims.of_int (131)) (Prims.of_int (35)))))
       (FStar_Sealed.seal
          (Obj.magic
-            (FStar_Range.mk_range "Pulse.Main.fst" (Prims.of_int (129))
-               (Prims.of_int (36)) (Prims.of_int (150)) (Prims.of_int (4)))))
+            (FStar_Range.mk_range "Pulse.Main.fst" (Prims.of_int (131))
+               (Prims.of_int (36)) (Prims.of_int (152)) (Prims.of_int (4)))))
       (Obj.magic
          (FStar_Tactics_Effect.tac_bind
             (FStar_Sealed.seal
                (Obj.magic
-                  (FStar_Range.mk_range "Pulse.Main.fst" (Prims.of_int (128))
-                     (Prims.of_int (5)) (Prims.of_int (128))
+                  (FStar_Range.mk_range "Pulse.Main.fst" (Prims.of_int (130))
+                     (Prims.of_int (5)) (Prims.of_int (130))
                      (Prims.of_int (48)))))
             (FStar_Sealed.seal
                (Obj.magic
-                  (FStar_Range.mk_range "Pulse.Main.fst" (Prims.of_int (128))
-                     (Prims.of_int (2)) (Prims.of_int (129))
+                  (FStar_Range.mk_range "Pulse.Main.fst" (Prims.of_int (130))
+                     (Prims.of_int (2)) (Prims.of_int (131))
                      (Prims.of_int (35)))))
             (Obj.magic
                (FStar_Tactics_Effect.tac_bind
                   (FStar_Sealed.seal
                      (Obj.magic
                         (FStar_Range.mk_range "Pulse.Main.fst"
-                           (Prims.of_int (128)) (Prims.of_int (23))
-                           (Prims.of_int (128)) (Prims.of_int (35)))))
+                           (Prims.of_int (130)) (Prims.of_int (23))
+                           (Prims.of_int (130)) (Prims.of_int (35)))))
                   (FStar_Sealed.seal
                      (Obj.magic
                         (FStar_Range.mk_range "Pulse.Main.fst"
-                           (Prims.of_int (128)) (Prims.of_int (5))
-                           (Prims.of_int (128)) (Prims.of_int (48)))))
+                           (Prims.of_int (130)) (Prims.of_int (5))
+                           (Prims.of_int (130)) (Prims.of_int (48)))))
                   (Obj.magic (FStar_Tactics_V2_Builtins.top_env ()))
                   (fun uu___1 ->
                      FStar_Tactics_Effect.lift_div_tac
@@ -1234,13 +1292,13 @@ let (join_smt_goals : unit -> (unit, unit) FStar_Tactics_Effect.tac_repr) =
                  (FStar_Sealed.seal
                     (Obj.magic
                        (FStar_Range.mk_range "Pulse.Main.fst"
-                          (Prims.of_int (132)) (Prims.of_int (18))
-                          (Prims.of_int (132)) (Prims.of_int (30)))))
+                          (Prims.of_int (134)) (Prims.of_int (18))
+                          (Prims.of_int (134)) (Prims.of_int (30)))))
                  (FStar_Sealed.seal
                     (Obj.magic
                        (FStar_Range.mk_range "Pulse.Main.fst"
-                          (Prims.of_int (133)) (Prims.of_int (2))
-                          (Prims.of_int (150)) (Prims.of_int (4)))))
+                          (Prims.of_int (135)) (Prims.of_int (2))
+                          (Prims.of_int (152)) (Prims.of_int (4)))))
                  (Obj.magic (FStar_Tactics_V2_Derived.smt_goals ()))
                  (fun uu___2 ->
                     (fun smt_goals ->
@@ -1249,30 +1307,30 @@ let (join_smt_goals : unit -> (unit, unit) FStar_Tactics_Effect.tac_repr) =
                             (FStar_Sealed.seal
                                (Obj.magic
                                   (FStar_Range.mk_range "Pulse.Main.fst"
-                                     (Prims.of_int (133)) (Prims.of_int (2))
-                                     (Prims.of_int (133)) (Prims.of_int (34)))))
+                                     (Prims.of_int (135)) (Prims.of_int (2))
+                                     (Prims.of_int (135)) (Prims.of_int (34)))))
                             (FStar_Sealed.seal
                                (Obj.magic
                                   (FStar_Range.mk_range "Pulse.Main.fst"
-                                     (Prims.of_int (134)) (Prims.of_int (2))
-                                     (Prims.of_int (150)) (Prims.of_int (4)))))
+                                     (Prims.of_int (136)) (Prims.of_int (2))
+                                     (Prims.of_int (152)) (Prims.of_int (4)))))
                             (Obj.magic
                                (FStar_Tactics_Effect.tac_bind
                                   (FStar_Sealed.seal
                                      (Obj.magic
                                         (FStar_Range.mk_range
                                            "Pulse.Main.fst"
-                                           (Prims.of_int (133))
+                                           (Prims.of_int (135))
                                            (Prims.of_int (12))
-                                           (Prims.of_int (133))
+                                           (Prims.of_int (135))
                                            (Prims.of_int (34)))))
                                   (FStar_Sealed.seal
                                      (Obj.magic
                                         (FStar_Range.mk_range
                                            "Pulse.Main.fst"
-                                           (Prims.of_int (133))
+                                           (Prims.of_int (135))
                                            (Prims.of_int (2))
-                                           (Prims.of_int (133))
+                                           (Prims.of_int (135))
                                            (Prims.of_int (34)))))
                                   (Obj.magic
                                      (FStar_Tactics_Effect.tac_bind
@@ -1280,17 +1338,17 @@ let (join_smt_goals : unit -> (unit, unit) FStar_Tactics_Effect.tac_repr) =
                                            (Obj.magic
                                               (FStar_Range.mk_range
                                                  "Pulse.Main.fst"
-                                                 (Prims.of_int (133))
+                                                 (Prims.of_int (135))
                                                  (Prims.of_int (13))
-                                                 (Prims.of_int (133))
+                                                 (Prims.of_int (135))
                                                  (Prims.of_int (21)))))
                                         (FStar_Sealed.seal
                                            (Obj.magic
                                               (FStar_Range.mk_range
                                                  "Pulse.Main.fst"
-                                                 (Prims.of_int (133))
+                                                 (Prims.of_int (135))
                                                  (Prims.of_int (12))
-                                                 (Prims.of_int (133))
+                                                 (Prims.of_int (135))
                                                  (Prims.of_int (34)))))
                                         (Obj.magic
                                            (FStar_Tactics_V2_Derived.goals ()))
@@ -1312,17 +1370,17 @@ let (join_smt_goals : unit -> (unit, unit) FStar_Tactics_Effect.tac_repr) =
                                           (Obj.magic
                                              (FStar_Range.mk_range
                                                 "Pulse.Main.fst"
-                                                (Prims.of_int (134))
+                                                (Prims.of_int (136))
                                                 (Prims.of_int (2))
-                                                (Prims.of_int (134))
+                                                (Prims.of_int (136))
                                                 (Prims.of_int (18)))))
                                        (FStar_Sealed.seal
                                           (Obj.magic
                                              (FStar_Range.mk_range
                                                 "Pulse.Main.fst"
-                                                (Prims.of_int (134))
+                                                (Prims.of_int (136))
                                                 (Prims.of_int (19))
-                                                (Prims.of_int (150))
+                                                (Prims.of_int (152))
                                                 (Prims.of_int (4)))))
                                        (Obj.magic
                                           (FStar_Tactics_V2_Builtins.set_smt_goals
@@ -1335,17 +1393,17 @@ let (join_smt_goals : unit -> (unit, unit) FStar_Tactics_Effect.tac_repr) =
                                                      (Obj.magic
                                                         (FStar_Range.mk_range
                                                            "Pulse.Main.fst"
-                                                           (Prims.of_int (135))
+                                                           (Prims.of_int (137))
                                                            (Prims.of_int (10))
-                                                           (Prims.of_int (135))
+                                                           (Prims.of_int (137))
                                                            (Prims.of_int (36)))))
                                                   (FStar_Sealed.seal
                                                      (Obj.magic
                                                         (FStar_Range.mk_range
                                                            "Pulse.Main.fst"
-                                                           (Prims.of_int (136))
+                                                           (Prims.of_int (138))
                                                            (Prims.of_int (2))
-                                                           (Prims.of_int (150))
+                                                           (Prims.of_int (152))
                                                            (Prims.of_int (4)))))
                                                   (Obj.magic
                                                      (FStar_Tactics_Effect.tac_bind
@@ -1353,17 +1411,17 @@ let (join_smt_goals : unit -> (unit, unit) FStar_Tactics_Effect.tac_repr) =
                                                            (Obj.magic
                                                               (FStar_Range.mk_range
                                                                  "Pulse.Main.fst"
-                                                                 (Prims.of_int (135))
+                                                                 (Prims.of_int (137))
                                                                  (Prims.of_int (26))
-                                                                 (Prims.of_int (135))
+                                                                 (Prims.of_int (137))
                                                                  (Prims.of_int (36)))))
                                                         (FStar_Sealed.seal
                                                            (Obj.magic
                                                               (FStar_Range.mk_range
                                                                  "Pulse.Main.fst"
-                                                                 (Prims.of_int (135))
+                                                                 (Prims.of_int (137))
                                                                  (Prims.of_int (10))
-                                                                 (Prims.of_int (135))
+                                                                 (Prims.of_int (137))
                                                                  (Prims.of_int (36)))))
                                                         (Obj.magic
                                                            (FStar_Tactics_V2_Derived.goals
@@ -1381,17 +1439,17 @@ let (join_smt_goals : unit -> (unit, unit) FStar_Tactics_Effect.tac_repr) =
                                                                 (Obj.magic
                                                                    (FStar_Range.mk_range
                                                                     "Pulse.Main.fst"
-                                                                    (Prims.of_int (136))
+                                                                    (Prims.of_int (138))
                                                                     (Prims.of_int (2))
-                                                                    (Prims.of_int (136))
+                                                                    (Prims.of_int (138))
                                                                     (Prims.of_int (22)))))
                                                              (FStar_Sealed.seal
                                                                 (Obj.magic
                                                                    (FStar_Range.mk_range
                                                                     "Pulse.Main.fst"
-                                                                    (Prims.of_int (141))
+                                                                    (Prims.of_int (143))
                                                                     (Prims.of_int (2))
-                                                                    (Prims.of_int (150))
+                                                                    (Prims.of_int (152))
                                                                     (Prims.of_int (4)))))
                                                              (Obj.magic
                                                                 (FStar_Tactics_Effect.tac_bind
@@ -1399,17 +1457,17 @@ let (join_smt_goals : unit -> (unit, unit) FStar_Tactics_Effect.tac_repr) =
                                                                     (Obj.magic
                                                                     (FStar_Range.mk_range
                                                                     "Pulse.Main.fst"
-                                                                    (Prims.of_int (136))
+                                                                    (Prims.of_int (138))
                                                                     (Prims.of_int (9))
-                                                                    (Prims.of_int (136))
+                                                                    (Prims.of_int (138))
                                                                     (Prims.of_int (22)))))
                                                                    (FStar_Sealed.seal
                                                                     (Obj.magic
                                                                     (FStar_Range.mk_range
                                                                     "Pulse.Main.fst"
-                                                                    (Prims.of_int (136))
+                                                                    (Prims.of_int (138))
                                                                     (Prims.of_int (2))
-                                                                    (Prims.of_int (136))
+                                                                    (Prims.of_int (138))
                                                                     (Prims.of_int (22)))))
                                                                    (Obj.magic
                                                                     (FStar_Tactics_V2_Derived.repeat
@@ -1429,17 +1487,17 @@ let (join_smt_goals : unit -> (unit, unit) FStar_Tactics_Effect.tac_repr) =
                                                                     (Obj.magic
                                                                     (FStar_Range.mk_range
                                                                     "Pulse.Main.fst"
-                                                                    (Prims.of_int (141))
+                                                                    (Prims.of_int (143))
                                                                     (Prims.of_int (2))
-                                                                    (Prims.of_int (145))
+                                                                    (Prims.of_int (147))
                                                                     (Prims.of_int (3)))))
                                                                     (FStar_Sealed.seal
                                                                     (Obj.magic
                                                                     (FStar_Range.mk_range
                                                                     "Pulse.Main.fst"
-                                                                    (Prims.of_int (147))
+                                                                    (Prims.of_int (149))
                                                                     (Prims.of_int (2))
-                                                                    (Prims.of_int (150))
+                                                                    (Prims.of_int (152))
                                                                     (Prims.of_int (4)))))
                                                                     (Obj.magic
                                                                     (FStar_Tactics_Effect.tac_bind
@@ -1447,17 +1505,17 @@ let (join_smt_goals : unit -> (unit, unit) FStar_Tactics_Effect.tac_repr) =
                                                                     (Obj.magic
                                                                     (FStar_Range.mk_range
                                                                     "Pulse.Main.fst"
-                                                                    (Prims.of_int (141))
+                                                                    (Prims.of_int (143))
                                                                     (Prims.of_int (5))
-                                                                    (Prims.of_int (141))
+                                                                    (Prims.of_int (143))
                                                                     (Prims.of_int (26)))))
                                                                     (FStar_Sealed.seal
                                                                     (Obj.magic
                                                                     (FStar_Range.mk_range
                                                                     "Pulse.Main.fst"
-                                                                    (Prims.of_int (141))
+                                                                    (Prims.of_int (143))
                                                                     (Prims.of_int (2))
-                                                                    (Prims.of_int (145))
+                                                                    (Prims.of_int (147))
                                                                     (Prims.of_int (3)))))
                                                                     (Obj.magic
                                                                     (FStar_Tactics_Effect.tac_bind
@@ -1465,17 +1523,17 @@ let (join_smt_goals : unit -> (unit, unit) FStar_Tactics_Effect.tac_repr) =
                                                                     (Obj.magic
                                                                     (FStar_Range.mk_range
                                                                     "Pulse.Main.fst"
-                                                                    (Prims.of_int (141))
+                                                                    (Prims.of_int (143))
                                                                     (Prims.of_int (9))
-                                                                    (Prims.of_int (141))
+                                                                    (Prims.of_int (143))
                                                                     (Prims.of_int (26)))))
                                                                     (FStar_Sealed.seal
                                                                     (Obj.magic
                                                                     (FStar_Range.mk_range
                                                                     "Pulse.Main.fst"
-                                                                    (Prims.of_int (141))
+                                                                    (Prims.of_int (143))
                                                                     (Prims.of_int (5))
-                                                                    (Prims.of_int (141))
+                                                                    (Prims.of_int (143))
                                                                     (Prims.of_int (26)))))
                                                                     (Obj.magic
                                                                     (FStar_Tactics_Effect.tac_bind
@@ -1483,17 +1541,17 @@ let (join_smt_goals : unit -> (unit, unit) FStar_Tactics_Effect.tac_repr) =
                                                                     (Obj.magic
                                                                     (FStar_Range.mk_range
                                                                     "Pulse.Main.fst"
-                                                                    (Prims.of_int (141))
+                                                                    (Prims.of_int (143))
                                                                     (Prims.of_int (15))
-                                                                    (Prims.of_int (141))
+                                                                    (Prims.of_int (143))
                                                                     (Prims.of_int (25)))))
                                                                     (FStar_Sealed.seal
                                                                     (Obj.magic
                                                                     (FStar_Range.mk_range
                                                                     "Pulse.Main.fst"
-                                                                    (Prims.of_int (141))
+                                                                    (Prims.of_int (143))
                                                                     (Prims.of_int (9))
-                                                                    (Prims.of_int (141))
+                                                                    (Prims.of_int (143))
                                                                     (Prims.of_int (26)))))
                                                                     (Obj.magic
                                                                     (FStar_Tactics_V2_Derived.goals
@@ -1525,17 +1583,17 @@ let (join_smt_goals : unit -> (unit, unit) FStar_Tactics_Effect.tac_repr) =
                                                                     (Obj.magic
                                                                     (FStar_Range.mk_range
                                                                     "Pulse.Main.fst"
-                                                                    (Prims.of_int (143))
+                                                                    (Prims.of_int (145))
                                                                     (Prims.of_int (17))
-                                                                    (Prims.of_int (143))
+                                                                    (Prims.of_int (145))
                                                                     (Prims.of_int (39)))))
                                                                     (FStar_Sealed.seal
                                                                     (Obj.magic
                                                                     (FStar_Range.mk_range
                                                                     "Pulse.Main.fst"
-                                                                    (Prims.of_int (144))
+                                                                    (Prims.of_int (146))
                                                                     (Prims.of_int (4))
-                                                                    (Prims.of_int (144))
+                                                                    (Prims.of_int (146))
                                                                     (Prims.of_int (21)))))
                                                                     (Obj.magic
                                                                     (FStar_Tactics_Effect.tac_bind
@@ -1543,17 +1601,17 @@ let (join_smt_goals : unit -> (unit, unit) FStar_Tactics_Effect.tac_repr) =
                                                                     (Obj.magic
                                                                     (FStar_Range.mk_range
                                                                     "Pulse.Main.fst"
-                                                                    (Prims.of_int (143))
+                                                                    (Prims.of_int (145))
                                                                     (Prims.of_int (17))
-                                                                    (Prims.of_int (143))
+                                                                    (Prims.of_int (145))
                                                                     (Prims.of_int (29)))))
                                                                     (FStar_Sealed.seal
                                                                     (Obj.magic
                                                                     (FStar_Range.mk_range
                                                                     "Pulse.Main.fst"
-                                                                    (Prims.of_int (143))
+                                                                    (Prims.of_int (145))
                                                                     (Prims.of_int (17))
-                                                                    (Prims.of_int (143))
+                                                                    (Prims.of_int (145))
                                                                     (Prims.of_int (39)))))
                                                                     (Obj.magic
                                                                     (FStar_Tactics_SMT.get_rlimit
@@ -1594,17 +1652,17 @@ let (join_smt_goals : unit -> (unit, unit) FStar_Tactics_Effect.tac_repr) =
                                                                     (Obj.magic
                                                                     (FStar_Range.mk_range
                                                                     "Pulse.Main.fst"
-                                                                    (Prims.of_int (147))
+                                                                    (Prims.of_int (149))
                                                                     (Prims.of_int (2))
-                                                                    (Prims.of_int (148))
+                                                                    (Prims.of_int (150))
                                                                     (Prims.of_int (34)))))
                                                                     (FStar_Sealed.seal
                                                                     (Obj.magic
                                                                     (FStar_Range.mk_range
                                                                     "Pulse.Main.fst"
-                                                                    (Prims.of_int (150))
+                                                                    (Prims.of_int (152))
                                                                     (Prims.of_int (2))
-                                                                    (Prims.of_int (150))
+                                                                    (Prims.of_int (152))
                                                                     (Prims.of_int (4)))))
                                                                     (Obj.magic
                                                                     (FStar_Tactics_Effect.tac_bind
@@ -1612,17 +1670,17 @@ let (join_smt_goals : unit -> (unit, unit) FStar_Tactics_Effect.tac_repr) =
                                                                     (Obj.magic
                                                                     (FStar_Range.mk_range
                                                                     "Pulse.Main.fst"
-                                                                    (Prims.of_int (147))
+                                                                    (Prims.of_int (149))
                                                                     (Prims.of_int (5))
-                                                                    (Prims.of_int (147))
+                                                                    (Prims.of_int (149))
                                                                     (Prims.of_int (48)))))
                                                                     (FStar_Sealed.seal
                                                                     (Obj.magic
                                                                     (FStar_Range.mk_range
                                                                     "Pulse.Main.fst"
-                                                                    (Prims.of_int (147))
+                                                                    (Prims.of_int (149))
                                                                     (Prims.of_int (2))
-                                                                    (Prims.of_int (148))
+                                                                    (Prims.of_int (150))
                                                                     (Prims.of_int (34)))))
                                                                     (Obj.magic
                                                                     (FStar_Tactics_Effect.tac_bind
@@ -1630,17 +1688,17 @@ let (join_smt_goals : unit -> (unit, unit) FStar_Tactics_Effect.tac_repr) =
                                                                     (Obj.magic
                                                                     (FStar_Range.mk_range
                                                                     "Pulse.Main.fst"
-                                                                    (Prims.of_int (147))
+                                                                    (Prims.of_int (149))
                                                                     (Prims.of_int (23))
-                                                                    (Prims.of_int (147))
+                                                                    (Prims.of_int (149))
                                                                     (Prims.of_int (35)))))
                                                                     (FStar_Sealed.seal
                                                                     (Obj.magic
                                                                     (FStar_Range.mk_range
                                                                     "Pulse.Main.fst"
-                                                                    (Prims.of_int (147))
+                                                                    (Prims.of_int (149))
                                                                     (Prims.of_int (5))
-                                                                    (Prims.of_int (147))
+                                                                    (Prims.of_int (149))
                                                                     (Prims.of_int (48)))))
                                                                     (Obj.magic
                                                                     (FStar_Tactics_V2_Builtins.top_env
@@ -1693,38 +1751,38 @@ let (main :
           FStar_Tactics_Effect.tac_bind
             (FStar_Sealed.seal
                (Obj.magic
-                  (FStar_Range.mk_range "Pulse.Main.fst" (Prims.of_int (157))
-                     (Prims.of_int (2)) (Prims.of_int (160))
+                  (FStar_Range.mk_range "Pulse.Main.fst" (Prims.of_int (159))
+                     (Prims.of_int (2)) (Prims.of_int (162))
                      (Prims.of_int (24)))))
             (FStar_Sealed.seal
                (Obj.magic
-                  (FStar_Range.mk_range "Pulse.Main.fst" (Prims.of_int (160))
-                     (Prims.of_int (25)) (Prims.of_int (169))
+                  (FStar_Range.mk_range "Pulse.Main.fst" (Prims.of_int (162))
+                     (Prims.of_int (25)) (Prims.of_int (171))
                      (Prims.of_int (5)))))
             (Obj.magic
                (FStar_Tactics_Effect.tac_bind
                   (FStar_Sealed.seal
                      (Obj.magic
                         (FStar_Range.mk_range "Pulse.Main.fst"
-                           (Prims.of_int (157)) (Prims.of_int (5))
-                           (Prims.of_int (157)) (Prims.of_int (46)))))
+                           (Prims.of_int (159)) (Prims.of_int (5))
+                           (Prims.of_int (159)) (Prims.of_int (46)))))
                   (FStar_Sealed.seal
                      (Obj.magic
                         (FStar_Range.mk_range "Pulse.Main.fst"
-                           (Prims.of_int (157)) (Prims.of_int (2))
-                           (Prims.of_int (160)) (Prims.of_int (24)))))
+                           (Prims.of_int (159)) (Prims.of_int (2))
+                           (Prims.of_int (162)) (Prims.of_int (24)))))
                   (Obj.magic
                      (FStar_Tactics_Effect.tac_bind
                         (FStar_Sealed.seal
                            (Obj.magic
                               (FStar_Range.mk_range "Pulse.Main.fst"
-                                 (Prims.of_int (157)) (Prims.of_int (5))
-                                 (Prims.of_int (157)) (Prims.of_int (34)))))
+                                 (Prims.of_int (159)) (Prims.of_int (5))
+                                 (Prims.of_int (159)) (Prims.of_int (34)))))
                         (FStar_Sealed.seal
                            (Obj.magic
                               (FStar_Range.mk_range "Pulse.Main.fst"
-                                 (Prims.of_int (157)) (Prims.of_int (5))
-                                 (Prims.of_int (157)) (Prims.of_int (46)))))
+                                 (Prims.of_int (159)) (Prims.of_int (5))
+                                 (Prims.of_int (159)) (Prims.of_int (46)))))
                         (Obj.magic
                            (FStar_Tactics_V2_Builtins.ext_getv
                               "pulse:guard_policy"))
@@ -1749,13 +1807,13 @@ let (main :
                        (FStar_Sealed.seal
                           (Obj.magic
                              (FStar_Range.mk_range "Pulse.Main.fst"
-                                (Prims.of_int (162)) (Prims.of_int (12))
-                                (Prims.of_int (162)) (Prims.of_int (28)))))
+                                (Prims.of_int (164)) (Prims.of_int (12))
+                                (Prims.of_int (164)) (Prims.of_int (28)))))
                        (FStar_Sealed.seal
                           (Obj.magic
                              (FStar_Range.mk_range "Pulse.Main.fst"
-                                (Prims.of_int (164)) (Prims.of_int (2))
-                                (Prims.of_int (169)) (Prims.of_int (5)))))
+                                (Prims.of_int (166)) (Prims.of_int (2))
+                                (Prims.of_int (171)) (Prims.of_int (5)))))
                        (Obj.magic (main' nm t pre g))
                        (fun uu___1 ->
                           (fun res ->
@@ -1765,17 +1823,17 @@ let (main :
                                      (Obj.magic
                                         (FStar_Range.mk_range
                                            "Pulse.Main.fst"
-                                           (Prims.of_int (164))
+                                           (Prims.of_int (166))
                                            (Prims.of_int (2))
-                                           (Prims.of_int (168))
+                                           (Prims.of_int (170))
                                            (Prims.of_int (20)))))
                                   (FStar_Sealed.seal
                                      (Obj.magic
                                         (FStar_Range.mk_range
                                            "Pulse.Main.fst"
-                                           (Prims.of_int (162))
+                                           (Prims.of_int (164))
                                            (Prims.of_int (6))
-                                           (Prims.of_int (162))
+                                           (Prims.of_int (164))
                                            (Prims.of_int (9)))))
                                   (Obj.magic
                                      (FStar_Tactics_Effect.tac_bind
@@ -1783,17 +1841,17 @@ let (main :
                                            (Obj.magic
                                               (FStar_Range.mk_range
                                                  "Pulse.Main.fst"
-                                                 (Prims.of_int (164))
+                                                 (Prims.of_int (166))
                                                  (Prims.of_int (5))
-                                                 (Prims.of_int (164))
+                                                 (Prims.of_int (166))
                                                  (Prims.of_int (32)))))
                                         (FStar_Sealed.seal
                                            (Obj.magic
                                               (FStar_Range.mk_range
                                                  "Pulse.Main.fst"
-                                                 (Prims.of_int (164))
+                                                 (Prims.of_int (166))
                                                  (Prims.of_int (2))
-                                                 (Prims.of_int (168))
+                                                 (Prims.of_int (170))
                                                  (Prims.of_int (20)))))
                                         (Obj.magic
                                            (FStar_Tactics_Effect.tac_bind
@@ -1801,17 +1859,17 @@ let (main :
                                                  (Obj.magic
                                                     (FStar_Range.mk_range
                                                        "Pulse.Main.fst"
-                                                       (Prims.of_int (164))
+                                                       (Prims.of_int (166))
                                                        (Prims.of_int (5))
-                                                       (Prims.of_int (164))
+                                                       (Prims.of_int (166))
                                                        (Prims.of_int (26)))))
                                               (FStar_Sealed.seal
                                                  (Obj.magic
                                                     (FStar_Range.mk_range
                                                        "Pulse.Main.fst"
-                                                       (Prims.of_int (164))
+                                                       (Prims.of_int (166))
                                                        (Prims.of_int (5))
-                                                       (Prims.of_int (164))
+                                                       (Prims.of_int (166))
                                                        (Prims.of_int (32)))))
                                               (Obj.magic
                                                  (FStar_Tactics_V2_Builtins.ext_getv
@@ -1856,13 +1914,13 @@ let (check_pulse :
                     (FStar_Sealed.seal
                        (Obj.magic
                           (FStar_Range.mk_range "Pulse.Main.fst"
-                             (Prims.of_int (180)) (Prims.of_int (12))
-                             (Prims.of_int (180)) (Prims.of_int (112)))))
+                             (Prims.of_int (182)) (Prims.of_int (12))
+                             (Prims.of_int (182)) (Prims.of_int (112)))))
                     (FStar_Sealed.seal
                        (Obj.magic
                           (FStar_Range.mk_range "Pulse.Main.fst"
-                             (Prims.of_int (180)) (Prims.of_int (6))
-                             (Prims.of_int (196)) (Prims.of_int (36)))))
+                             (Prims.of_int (182)) (Prims.of_int (6))
+                             (Prims.of_int (198)) (Prims.of_int (36)))))
                     (FStar_Tactics_Effect.lift_div_tac
                        (fun uu___ ->
                           PulseSyntaxExtension_ASTBuilder.parse_pulse env
@@ -1890,17 +1948,17 @@ let (check_pulse :
                                          (Obj.magic
                                             (FStar_Range.mk_range
                                                "Pulse.Main.fst"
-                                               (Prims.of_int (189))
+                                               (Prims.of_int (191))
                                                (Prims.of_int (10))
-                                               (Prims.of_int (193))
+                                               (Prims.of_int (195))
                                                (Prims.of_int (21)))))
                                       (FStar_Sealed.seal
                                          (Obj.magic
                                             (FStar_Range.mk_range
                                                "Pulse.Main.fst"
-                                               (Prims.of_int (195))
+                                               (Prims.of_int (197))
                                                (Prims.of_int (8))
-                                               (Prims.of_int (196))
+                                               (Prims.of_int (198))
                                                (Prims.of_int (36)))))
                                       (Obj.magic
                                          (FStar_Tactics_Effect.tac_bind
@@ -1908,9 +1966,9 @@ let (check_pulse :
                                                (Obj.magic
                                                   (FStar_Range.mk_range
                                                      "Pulse.Main.fst"
-                                                     (Prims.of_int (190))
+                                                     (Prims.of_int (192))
                                                      (Prims.of_int (19))
-                                                     (Prims.of_int (190))
+                                                     (Prims.of_int (192))
                                                      (Prims.of_int (74)))))
                                             (FStar_Sealed.seal
                                                (Obj.magic
@@ -1926,17 +1984,17 @@ let (check_pulse :
                                                      (Obj.magic
                                                         (FStar_Range.mk_range
                                                            "Pulse.Main.fst"
-                                                           (Prims.of_int (190))
+                                                           (Prims.of_int (192))
                                                            (Prims.of_int (19))
-                                                           (Prims.of_int (190))
+                                                           (Prims.of_int (192))
                                                            (Prims.of_int (74)))))
                                                   (FStar_Sealed.seal
                                                      (Obj.magic
                                                         (FStar_Range.mk_range
                                                            "Pulse.Main.fst"
-                                                           (Prims.of_int (190))
+                                                           (Prims.of_int (192))
                                                            (Prims.of_int (19))
-                                                           (Prims.of_int (190))
+                                                           (Prims.of_int (192))
                                                            (Prims.of_int (74)))))
                                                   (Obj.magic
                                                      (FStar_Tactics_Effect.tac_bind
@@ -1944,9 +2002,9 @@ let (check_pulse :
                                                            (Obj.magic
                                                               (FStar_Range.mk_range
                                                                  "Pulse.Main.fst"
-                                                                 (Prims.of_int (190))
+                                                                 (Prims.of_int (192))
                                                                  (Prims.of_int (44))
-                                                                 (Prims.of_int (190))
+                                                                 (Prims.of_int (192))
                                                                  (Prims.of_int (69)))))
                                                         (FStar_Sealed.seal
                                                            (Obj.magic
@@ -1996,17 +2054,17 @@ let (check_pulse :
                                                     (Obj.magic
                                                        (FStar_Range.mk_range
                                                           "Pulse.Main.fst"
-                                                          (Prims.of_int (195))
+                                                          (Prims.of_int (197))
                                                           (Prims.of_int (8))
-                                                          (Prims.of_int (195))
+                                                          (Prims.of_int (197))
                                                           (Prims.of_int (24)))))
                                                  (FStar_Sealed.seal
                                                     (Obj.magic
                                                        (FStar_Range.mk_range
                                                           "Pulse.Main.fst"
-                                                          (Prims.of_int (196))
+                                                          (Prims.of_int (198))
                                                           (Prims.of_int (8))
-                                                          (Prims.of_int (196))
+                                                          (Prims.of_int (198))
                                                           (Prims.of_int (36)))))
                                                  (Obj.magic
                                                     (FStar_Tactics_V2_Builtins.log_issues
