pulse/src/ocaml/plugin/generated/Pulse_Syntax_Base.ml
@@ -252,7 +252,7 @@ and proof_hint_type =
   | RENAME of proof_hint_type__RENAME__payload 
   | REWRITE of proof_hint_type__REWRITE__payload 
   | WILD 
-  | SHOW_PROOF_STATE of FStar_Range.range 
+  | SHOW_PROOF_STATE of range 
 let (__proj__Mkproof_hint_type__ASSERT__payload__item__p :
   proof_hint_type__ASSERT__payload -> vprop) =
   fun projectee -> match projectee with | { p;_} -> p
@@ -314,8 +314,7 @@ let (uu___is_WILD : proof_hint_type -> Prims.bool) =
 let (uu___is_SHOW_PROOF_STATE : proof_hint_type -> Prims.bool) =
   fun projectee ->
     match projectee with | SHOW_PROOF_STATE _0 -> true | uu___ -> false
-let (__proj__SHOW_PROOF_STATE__item___0 :
-  proof_hint_type -> FStar_Range.range) =
+let (__proj__SHOW_PROOF_STATE__item___0 : proof_hint_type -> range) =
   fun projectee -> match projectee with | SHOW_PROOF_STATE _0 -> _0
 type comp_ascription =
   {
