pulse/src/ocaml/plugin/generated/Pulse_Typing_Combinators.ml
@@ -57,14 +57,14 @@ let rec (mk_bind :
                                (Obj.magic
                                   (FStar_Range.mk_range
                                      "Pulse.Typing.Combinators.fst"
-                                     (Prims.of_int (121)) (Prims.of_int (13))
-                                     (Prims.of_int (121)) (Prims.of_int (15)))))
+                                     (Prims.of_int (150)) (Prims.of_int (13))
+                                     (Prims.of_int (150)) (Prims.of_int (15)))))
                             (FStar_Sealed.seal
                                (Obj.magic
                                   (FStar_Range.mk_range
                                      "Pulse.Typing.Combinators.fst"
-                                     (Prims.of_int (120)) (Prims.of_int (38))
-                                     (Prims.of_int (201)) (Prims.of_int (82)))))
+                                     (Prims.of_int (149)) (Prims.of_int (38))
+                                     (Prims.of_int (230)) (Prims.of_int (82)))))
                             (FStar_Tactics_Effect.lift_div_tac
                                (fun uu___ -> px))
                             (fun uu___ ->
@@ -77,17 +77,17 @@ let rec (mk_bind :
                                               (Obj.magic
                                                  (FStar_Range.mk_range
                                                     "Pulse.Typing.Combinators.fst"
-                                                    (Prims.of_int (122))
+                                                    (Prims.of_int (151))
                                                     (Prims.of_int (10))
-                                                    (Prims.of_int (122))
+                                                    (Prims.of_int (151))
                                                     (Prims.of_int (41)))))
                                            (FStar_Sealed.seal
                                               (Obj.magic
                                                  (FStar_Range.mk_range
                                                     "Pulse.Typing.Combinators.fst"
-                                                    (Prims.of_int (123))
+                                                    (Prims.of_int (152))
                                                     (Prims.of_int (2))
-                                                    (Prims.of_int (201))
+                                                    (Prims.of_int (230))
                                                     (Prims.of_int (82)))))
                                            (FStar_Tactics_Effect.lift_div_tac
                                               (fun uu___2 ->
@@ -189,17 +189,17 @@ let rec (mk_bind :
                                                                     (Obj.magic
                                                                     (FStar_Range.mk_range
                                                                     "Pulse.Typing.Combinators.fst"
-                                                                    (Prims.of_int (133))
+                                                                    (Prims.of_int (162))
                                                                     (Prims.of_int (23))
-                                                                    (Prims.of_int (133))
+                                                                    (Prims.of_int (162))
                                                                     (Prims.of_int (53)))))
                                                                   (FStar_Sealed.seal
                                                                     (Obj.magic
                                                                     (FStar_Range.mk_range
                                                                     "Pulse.Typing.Combinators.fst"
-                                                                    (Prims.of_int (133))
+                                                                    (Prims.of_int (162))
                                                                     (Prims.of_int (56))
-                                                                    (Prims.of_int (139))
+                                                                    (Prims.of_int (168))
                                                                     (Prims.of_int (63)))))
                                                                   (FStar_Tactics_Effect.lift_div_tac
                                                                     (fun
@@ -218,17 +218,17 @@ let rec (mk_bind :
                                                                     (Obj.magic
                                                                     (FStar_Range.mk_range
                                                                     "Pulse.Typing.Combinators.fst"
-                                                                    (Prims.of_int (134))
+                                                                    (Prims.of_int (163))
                                                                     (Prims.of_int (17))
-                                                                    (Prims.of_int (134))
+                                                                    (Prims.of_int (163))
                                                                     (Prims.of_int (134)))))
                                                                     (FStar_Sealed.seal
                                                                     (Obj.magic
                                                                     (FStar_Range.mk_range
                                                                     "Pulse.Typing.Combinators.fst"
-                                                                    (Prims.of_int (134))
+                                                                    (Prims.of_int (163))
                                                                     (Prims.of_int (137))
-                                                                    (Prims.of_int (139))
+                                                                    (Prims.of_int (168))
                                                                     (Prims.of_int (63)))))
                                                                     (Obj.magic
                                                                     (FStar_Tactics_Effect.tac_bind
@@ -236,17 +236,17 @@ let rec (mk_bind :
                                                                     (Obj.magic
                                                                     (FStar_Range.mk_range
                                                                     "Pulse.Typing.Combinators.fst"
-                                                                    (Prims.of_int (134))
+                                                                    (Prims.of_int (163))
                                                                     (Prims.of_int (36))
-                                                                    (Prims.of_int (134))
+                                                                    (Prims.of_int (163))
                                                                     (Prims.of_int (134)))))
                                                                     (FStar_Sealed.seal
                                                                     (Obj.magic
                                                                     (FStar_Range.mk_range
                                                                     "Pulse.Typing.Combinators.fst"
-                                                                    (Prims.of_int (134))
+                                                                    (Prims.of_int (163))
                                                                     (Prims.of_int (17))
-                                                                    (Prims.of_int (134))
+                                                                    (Prims.of_int (163))
                                                                     (Prims.of_int (134)))))
                                                                     (Obj.magic
                                                                     (FStar_Tactics_Effect.tac_bind
@@ -254,17 +254,17 @@ let rec (mk_bind :
                                                                     (Obj.magic
                                                                     (FStar_Range.mk_range
                                                                     "Pulse.Typing.Combinators.fst"
-                                                                    (Prims.of_int (134))
+                                                                    (Prims.of_int (163))
                                                                     (Prims.of_int (76))
-                                                                    (Prims.of_int (134))
+                                                                    (Prims.of_int (163))
                                                                     (Prims.of_int (133)))))
                                                                     (FStar_Sealed.seal
                                                                     (Obj.magic
                                                                     (FStar_Range.mk_range
                                                                     "Pulse.Typing.Combinators.fst"
-                                                                    (Prims.of_int (134))
+                                                                    (Prims.of_int (163))
                                                                     (Prims.of_int (36))
-                                                                    (Prims.of_int (134))
+                                                                    (Prims.of_int (163))
                                                                     (Prims.of_int (134)))))
                                                                     (Obj.magic
                                                                     (Pulse_Checker_Pure.check_prop_validity
@@ -306,17 +306,17 @@ let rec (mk_bind :
                                                                     (Obj.magic
                                                                     (FStar_Range.mk_range
                                                                     "Pulse.Typing.Combinators.fst"
-                                                                    (Prims.of_int (135))
+                                                                    (Prims.of_int (164))
                                                                     (Prims.of_int (17))
-                                                                    (Prims.of_int (135))
+                                                                    (Prims.of_int (164))
                                                                     (Prims.of_int (134)))))
                                                                     (FStar_Sealed.seal
                                                                     (Obj.magic
                                                                     (FStar_Range.mk_range
                                                                     "Pulse.Typing.Combinators.fst"
-                                                                    (Prims.of_int (139))
+                                                                    (Prims.of_int (168))
                                                                     (Prims.of_int (6))
-                                                                    (Prims.of_int (139))
+                                                                    (Prims.of_int (168))
                                                                     (Prims.of_int (63)))))
                                                                     (Obj.magic
                                                                     (FStar_Tactics_Effect.tac_bind
@@ -324,17 +324,17 @@ let rec (mk_bind :
                                                                     (Obj.magic
                                                                     (FStar_Range.mk_range
                                                                     "Pulse.Typing.Combinators.fst"
-                                                                    (Prims.of_int (135))
+                                                                    (Prims.of_int (164))
                                                                     (Prims.of_int (36))
-                                                                    (Prims.of_int (135))
+                                                                    (Prims.of_int (164))
                                                                     (Prims.of_int (134)))))
                                                                     (FStar_Sealed.seal
                                                                     (Obj.magic
                                                                     (FStar_Range.mk_range
                                                                     "Pulse.Typing.Combinators.fst"
-                                                                    (Prims.of_int (135))
+                                                                    (Prims.of_int (164))
                                                                     (Prims.of_int (17))
-                                                                    (Prims.of_int (135))
+                                                                    (Prims.of_int (164))
                                                                     (Prims.of_int (134)))))
                                                                     (Obj.magic
                                                                     (FStar_Tactics_Effect.tac_bind
@@ -342,17 +342,17 @@ let rec (mk_bind :
                                                                     (Obj.magic
                                                                     (FStar_Range.mk_range
                                                                     "Pulse.Typing.Combinators.fst"
-                                                                    (Prims.of_int (135))
+                                                                    (Prims.of_int (164))
                                                                     (Prims.of_int (76))
-                                                                    (Prims.of_int (135))
+                                                                    (Prims.of_int (164))
                                                                     (Prims.of_int (133)))))
                                                                     (FStar_Sealed.seal
                                                                     (Obj.magic
                                                                     (FStar_Range.mk_range
                                                                     "Pulse.Typing.Combinators.fst"
-                                                                    (Prims.of_int (135))
+                                                                    (Prims.of_int (164))
                                                                     (Prims.of_int (36))
-                                                                    (Prims.of_int (135))
+                                                                    (Prims.of_int (164))
                                                                     (Prims.of_int (134)))))
                                                                     (Obj.magic
                                                                     (Pulse_Checker_Pure.check_prop_validity
@@ -546,17 +546,17 @@ let rec (mk_bind :
                                                                   (Obj.magic
                                                                     (FStar_Range.mk_range
                                                                     "Pulse.Typing.Combinators.fst"
-                                                                    (Prims.of_int (152))
+                                                                    (Prims.of_int (181))
                                                                     (Prims.of_int (14))
-                                                                    (Prims.of_int (152))
+                                                                    (Prims.of_int (181))
                                                                     (Prims.of_int (69)))))
                                                                (FStar_Sealed.seal
                                                                   (Obj.magic
                                                                     (FStar_Range.mk_range
                                                                     "Pulse.Typing.Combinators.fst"
-                                                                    (Prims.of_int (154))
+                                                                    (Prims.of_int (183))
                                                                     (Prims.of_int (6))
-                                                                    (Prims.of_int (154))
+                                                                    (Prims.of_int (183))
                                                                     (Prims.of_int (63)))))
                                                                (Obj.magic
                                                                   (Pulse_Checker_Pure.get_non_informative_witness
@@ -621,17 +621,17 @@ let rec (mk_bind :
                                                                   (Obj.magic
                                                                     (FStar_Range.mk_range
                                                                     "Pulse.Typing.Combinators.fst"
-                                                                    (Prims.of_int (160))
+                                                                    (Prims.of_int (189))
                                                                     (Prims.of_int (14))
-                                                                    (Prims.of_int (160))
+                                                                    (Prims.of_int (189))
                                                                     (Prims.of_int (69)))))
                                                                (FStar_Sealed.seal
                                                                   (Obj.magic
                                                                     (FStar_Range.mk_range
                                                                     "Pulse.Typing.Combinators.fst"
-                                                                    (Prims.of_int (162))
+                                                                    (Prims.of_int (191))
                                                                     (Prims.of_int (6))
-                                                                    (Prims.of_int (162))
+                                                                    (Prims.of_int (191))
                                                                     (Prims.of_int (63)))))
                                                                (Obj.magic
                                                                   (Pulse_Checker_Pure.get_non_informative_witness
@@ -782,17 +782,17 @@ let rec (mk_bind :
                                                                 (Obj.magic
                                                                    (FStar_Range.mk_range
                                                                     "Pulse.Typing.Combinators.fst"
-                                                                    (Prims.of_int (178))
+                                                                    (Prims.of_int (207))
                                                                     (Prims.of_int (14))
-                                                                    (Prims.of_int (178))
+                                                                    (Prims.of_int (207))
                                                                     (Prims.of_int (69)))))
                                                              (FStar_Sealed.seal
                                                                 (Obj.magic
                                                                    (FStar_Range.mk_range
                                                                     "Pulse.Typing.Combinators.fst"
-                                                                    (Prims.of_int (178))
+                                                                    (Prims.of_int (207))
                                                                     (Prims.of_int (72))
-                                                                    (Prims.of_int (182))
+                                                                    (Prims.of_int (211))
                                                                     (Prims.of_int (81)))))
                                                              (Obj.magic
                                                                 (Pulse_Checker_Pure.get_non_informative_witness
@@ -809,17 +809,17 @@ let rec (mk_bind :
                                                                     (Obj.magic
                                                                     (FStar_Range.mk_range
                                                                     "Pulse.Typing.Combinators.fst"
-                                                                    (Prims.of_int (179))
+                                                                    (Prims.of_int (208))
                                                                     (Prims.of_int (21))
-                                                                    (Prims.of_int (179))
+                                                                    (Prims.of_int (208))
                                                                     (Prims.of_int (59)))))
                                                                     (FStar_Sealed.seal
                                                                     (Obj.magic
                                                                     (FStar_Range.mk_range
                                                                     "Pulse.Typing.Combinators.fst"
-                                                                    (Prims.of_int (179))
+                                                                    (Prims.of_int (208))
                                                                     (Prims.of_int (62))
-                                                                    (Prims.of_int (182))
+                                                                    (Prims.of_int (211))
                                                                     (Prims.of_int (81)))))
                                                                     (FStar_Tactics_Effect.lift_div_tac
                                                                     (fun
@@ -839,17 +839,17 @@ let rec (mk_bind :
                                                                     (Obj.magic
                                                                     (FStar_Range.mk_range
                                                                     "Pulse.Typing.Combinators.fst"
-                                                                    (Prims.of_int (181))
+                                                                    (Prims.of_int (210))
                                                                     (Prims.of_int (8))
-                                                                    (Prims.of_int (181))
+                                                                    (Prims.of_int (210))
                                                                     (Prims.of_int (65)))))
                                                                     (FStar_Sealed.seal
                                                                     (Obj.magic
                                                                     (FStar_Range.mk_range
                                                                     "Pulse.Typing.Combinators.fst"
-                                                                    (Prims.of_int (182))
+                                                                    (Prims.of_int (211))
                                                                     (Prims.of_int (6))
-                                                                    (Prims.of_int (182))
+                                                                    (Prims.of_int (211))
                                                                     (Prims.of_int (81)))))
                                                                     (FStar_Tactics_Effect.lift_div_tac
                                                                     (fun
@@ -894,17 +894,17 @@ let rec (mk_bind :
                                                                   (Obj.magic
                                                                     (FStar_Range.mk_range
                                                                     "Pulse.Typing.Combinators.fst"
-                                                                    (Prims.of_int (187))
+                                                                    (Prims.of_int (216))
                                                                     (Prims.of_int (15))
-                                                                    (Prims.of_int (187))
+                                                                    (Prims.of_int (216))
                                                                     (Prims.of_int (54)))))
                                                                (FStar_Sealed.seal
                                                                   (Obj.magic
                                                                     (FStar_Range.mk_range
                                                                     "Pulse.Typing.Combinators.fst"
-                                                                    (Prims.of_int (187))
+                                                                    (Prims.of_int (216))
                                                                     (Prims.of_int (57))
-                                                                    (Prims.of_int (193))
+                                                                    (Prims.of_int (222))
                                                                     (Prims.of_int (19)))))
                                                                (FStar_Tactics_Effect.lift_div_tac
                                                                   (fun uu___4
@@ -923,17 +923,17 @@ let rec (mk_bind :
                                                                     (Obj.magic
                                                                     (FStar_Range.mk_range
                                                                     "Pulse.Typing.Combinators.fst"
-                                                                    (Prims.of_int (188))
+                                                                    (Prims.of_int (217))
                                                                     (Prims.of_int (14))
-                                                                    (Prims.of_int (188))
+                                                                    (Prims.of_int (217))
                                                                     (Prims.of_int (70)))))
                                                                     (FStar_Sealed.seal
                                                                     (Obj.magic
                                                                     (FStar_Range.mk_range
                                                                     "Pulse.Typing.Combinators.fst"
-                                                                    (Prims.of_int (188))
+                                                                    (Prims.of_int (217))
                                                                     (Prims.of_int (73))
-                                                                    (Prims.of_int (193))
+                                                                    (Prims.of_int (222))
                                                                     (Prims.of_int (19)))))
                                                                     (Obj.magic
                                                                     (Pulse_Checker_Pure.get_non_informative_witness
@@ -951,17 +951,17 @@ let rec (mk_bind :
                                                                     (Obj.magic
                                                                     (FStar_Range.mk_range
                                                                     "Pulse.Typing.Combinators.fst"
-                                                                    (Prims.of_int (189))
+                                                                    (Prims.of_int (218))
                                                                     (Prims.of_int (21))
-                                                                    (Prims.of_int (189))
+                                                                    (Prims.of_int (218))
                                                                     (Prims.of_int (59)))))
                                                                     (FStar_Sealed.seal
                                                                     (Obj.magic
                                                                     (FStar_Range.mk_range
                                                                     "Pulse.Typing.Combinators.fst"
-                                                                    (Prims.of_int (189))
+                                                                    (Prims.of_int (218))
                                                                     (Prims.of_int (62))
-                                                                    (Prims.of_int (193))
+                                                                    (Prims.of_int (222))
                                                                     (Prims.of_int (19)))))
                                                                     (FStar_Tactics_Effect.lift_div_tac
                                                                     (fun
@@ -981,17 +981,17 @@ let rec (mk_bind :
                                                                     (Obj.magic
                                                                     (FStar_Range.mk_range
                                                                     "Pulse.Typing.Combinators.fst"
-                                                                    (Prims.of_int (191))
+                                                                    (Prims.of_int (220))
                                                                     (Prims.of_int (8))
-                                                                    (Prims.of_int (191))
+                                                                    (Prims.of_int (220))
                                                                     (Prims.of_int (66)))))
                                                                     (FStar_Sealed.seal
                                                                     (Obj.magic
                                                                     (FStar_Range.mk_range
                                                                     "Pulse.Typing.Combinators.fst"
-                                                                    (Prims.of_int (191))
+                                                                    (Prims.of_int (220))
                                                                     (Prims.of_int (69))
-                                                                    (Prims.of_int (193))
+                                                                    (Prims.of_int (222))
                                                                     (Prims.of_int (19)))))
                                                                     (FStar_Tactics_Effect.lift_div_tac
                                                                     (fun
@@ -1023,17 +1023,17 @@ let rec (mk_bind :
                                                                     (Obj.magic
                                                                     (FStar_Range.mk_range
                                                                     "Pulse.Typing.Combinators.fst"
-                                                                    (Prims.of_int (192))
+                                                                    (Prims.of_int (221))
                                                                     (Prims.of_int (26))
-                                                                    (Prims.of_int (192))
+                                                                    (Prims.of_int (221))
                                                                     (Prims.of_int (101)))))
                                                                     (FStar_Sealed.seal
                                                                     (Obj.magic
                                                                     (FStar_Range.mk_range
                                                                     "Pulse.Typing.Combinators.fst"
-                                                                    (Prims.of_int (191))
+                                                                    (Prims.of_int (220))
                                                                     (Prims.of_int (69))
-                                                                    (Prims.of_int (193))
+                                                                    (Prims.of_int (222))
                                                                     (Prims.of_int (19)))))
                                                                     (Obj.magic
                                                                     (mk_bind
@@ -1076,17 +1076,17 @@ let rec (mk_bind :
                                                                 (Obj.magic
                                                                    (FStar_Range.mk_range
                                                                     "Pulse.Typing.Combinators.fst"
-                                                                    (Prims.of_int (197))
+                                                                    (Prims.of_int (226))
                                                                     (Prims.of_int (19))
-                                                                    (Prims.of_int (197))
+                                                                    (Prims.of_int (226))
                                                                     (Prims.of_int (44)))))
                                                              (FStar_Sealed.seal
                                                                 (Obj.magic
                                                                    (FStar_Range.mk_range
                                                                     "Pulse.Typing.Combinators.fst"
-                                                                    (Prims.of_int (197))
+                                                                    (Prims.of_int (226))
                                                                     (Prims.of_int (47))
-                                                                    (Prims.of_int (200))
+                                                                    (Prims.of_int (229))
                                                                     (Prims.of_int (79)))))
                                                              (FStar_Tactics_Effect.lift_div_tac
                                                                 (fun uu___5
@@ -1103,17 +1103,17 @@ let rec (mk_bind :
                                                                     (Obj.magic
                                                                     (FStar_Range.mk_range
                                                                     "Pulse.Typing.Combinators.fst"
-                                                                    (Prims.of_int (199))
+                                                                    (Prims.of_int (228))
                                                                     (Prims.of_int (6))
-                                                                    (Prims.of_int (199))
+                                                                    (Prims.of_int (228))
                                                                     (Prims.of_int (56)))))
                                                                     (FStar_Sealed.seal
                                                                     (Obj.magic
                                                                     (FStar_Range.mk_range
                                                                     "Pulse.Typing.Combinators.fst"
-                                                                    (Prims.of_int (200))
+                                                                    (Prims.of_int (229))
                                                                     (Prims.of_int (4))
-                                                                    (Prims.of_int (200))
+                                                                    (Prims.of_int (229))
                                                                     (Prims.of_int (79)))))
                                                                     (FStar_Tactics_Effect.lift_div_tac
                                                                     (fun
@@ -1172,17 +1172,17 @@ let (bind_res_and_post_typing :
                                   (Obj.magic
                                      (FStar_Range.mk_range
                                         "Pulse.Typing.Combinators.fst"
-                                        (Prims.of_int (213))
+                                        (Prims.of_int (242))
                                         (Prims.of_int (32))
-                                        (Prims.of_int (213))
+                                        (Prims.of_int (242))
                                         (Prims.of_int (55)))))
                                (FStar_Sealed.seal
                                   (Obj.magic
                                      (FStar_Range.mk_range
                                         "Pulse.Typing.Combinators.fst"
-                                        (Prims.of_int (210))
+                                        (Prims.of_int (239))
                                         (Prims.of_int (13))
-                                        (Prims.of_int (224))
+                                        (Prims.of_int (253))
                                         (Prims.of_int (7)))))
                                (Obj.magic
                                   (Pulse_Checker_Pure.check_universe g
@@ -1212,17 +1212,17 @@ let (bind_res_and_post_typing :
                                                      (Obj.magic
                                                         (FStar_Range.mk_range
                                                            "Pulse.Typing.Combinators.fst"
-                                                           (Prims.of_int (217))
+                                                           (Prims.of_int (246))
                                                            (Prims.of_int (23))
-                                                           (Prims.of_int (217))
+                                                           (Prims.of_int (246))
                                                            (Prims.of_int (122)))))
                                                   (FStar_Sealed.seal
                                                      (Obj.magic
                                                         (FStar_Range.mk_range
                                                            "Pulse.Typing.Combinators.fst"
-                                                           (Prims.of_int (217))
+                                                           (Prims.of_int (246))
                                                            (Prims.of_int (11))
-                                                           (Prims.of_int (217))
+                                                           (Prims.of_int (246))
                                                            (Prims.of_int (122)))))
                                                   (Obj.magic
                                                      (FStar_Tactics_Effect.tac_bind
@@ -1230,9 +1230,9 @@ let (bind_res_and_post_typing :
                                                            (Obj.magic
                                                               (FStar_Range.mk_range
                                                                  "Pulse.Typing.Combinators.fst"
-                                                                 (Prims.of_int (217))
+                                                                 (Prims.of_int (246))
                                                                  (Prims.of_int (95))
-                                                                 (Prims.of_int (217))
+                                                                 (Prims.of_int (246))
                                                                  (Prims.of_int (121)))))
                                                         (FStar_Sealed.seal
                                                            (Obj.magic
@@ -1271,17 +1271,17 @@ let (bind_res_and_post_typing :
                                                      (Obj.magic
                                                         (FStar_Range.mk_range
                                                            "Pulse.Typing.Combinators.fst"
-                                                           (Prims.of_int (219))
+                                                           (Prims.of_int (248))
                                                            (Prims.of_int (16))
-                                                           (Prims.of_int (219))
+                                                           (Prims.of_int (248))
                                                            (Prims.of_int (17)))))
                                                   (FStar_Sealed.seal
                                                      (Obj.magic
                                                         (FStar_Range.mk_range
                                                            "Pulse.Typing.Combinators.fst"
-                                                           (Prims.of_int (219))
+                                                           (Prims.of_int (248))
                                                            (Prims.of_int (20))
-                                                           (Prims.of_int (223))
+                                                           (Prims.of_int (252))
                                                            (Prims.of_int (31)))))
                                                   (FStar_Tactics_Effect.lift_div_tac
                                                      (fun uu___3 -> x))
@@ -1293,17 +1293,17 @@ let (bind_res_and_post_typing :
                                                                 (Obj.magic
                                                                    (FStar_Range.mk_range
                                                                     "Pulse.Typing.Combinators.fst"
-                                                                    (Prims.of_int (220))
+                                                                    (Prims.of_int (249))
                                                                     (Prims.of_int (29))
-                                                                    (Prims.of_int (220))
+                                                                    (Prims.of_int (249))
                                                                     (Prims.of_int (61)))))
                                                              (FStar_Sealed.seal
                                                                 (Obj.magic
                                                                    (FStar_Range.mk_range
                                                                     "Pulse.Typing.Combinators.fst"
-                                                                    (Prims.of_int (220))
+                                                                    (Prims.of_int (249))
                                                                     (Prims.of_int (64))
-                                                                    (Prims.of_int (223))
+                                                                    (Prims.of_int (252))
                                                                     (Prims.of_int (31)))))
                                                              (FStar_Tactics_Effect.lift_div_tac
                                                                 (fun uu___3
@@ -1322,17 +1322,17 @@ let (bind_res_and_post_typing :
                                                                     (Obj.magic
                                                                     (FStar_Range.mk_range
                                                                     "Pulse.Typing.Combinators.fst"
-                                                                    (Prims.of_int (222))
+                                                                    (Prims.of_int (251))
                                                                     (Prims.of_int (10))
-                                                                    (Prims.of_int (222))
+                                                                    (Prims.of_int (251))
                                                                     (Prims.of_int (87)))))
                                                                     (FStar_Sealed.seal
                                                                     (Obj.magic
                                                                     (FStar_Range.mk_range
                                                                     "Pulse.Typing.Combinators.fst"
-                                                                    (Prims.of_int (223))
+                                                                    (Prims.of_int (252))
                                                                     (Prims.of_int (8))
-                                                                    (Prims.of_int (223))
+                                                                    (Prims.of_int (252))
                                                                     (Prims.of_int (31)))))
                                                                     (Obj.magic
                                                                     (Pulse_Checker_Pure.check_vprop_with_core
