pulse/share/steel/examples/pulse/bug-reports/BugUnificationUnderBinder.fst
@@ -21,5 +21,26 @@ ensures emp
 {
     with zz. assert (forall* x. p x zz);
     drop_ _;
+} 
+```
+
+assume
+val is_list (l:list int) : vprop
+open FStar.List.Tot
+
+let aux (l1 l2:list 'a) (x:'a) 
+: Lemma 
+    (ensures l1@(x::l2) == (l1 @ [x])@l2)
+    [SMTPat (l1@(x::l2))]
+= List.Tot.Properties.append_assoc l1 [x] l2
+
+```pulse
+fn test1 (pfx:list int) (hd:int)
+requires forall* tl. is_list (pfx @ (hd::tl))
+ensures emp
+{
+    rewrite (forall* tl. is_list (pfx @ (hd::tl)))
+          as (forall* tl. is_list ((pfx @ [hd])@tl));
+    admit()
 }
 ```
